Removed sorry from beta_pr regularity

LogicalRefinement/Typed/Basic.lean
@@ -278,12 +278,12 @@ inductive HasType: Context -> Term -> Annot -> Prop
     HasType Γ (beta t s) 
     (proof (eq (B.subst0 t) 
     (app (pi A B) (lam A s) t) (s.subst0 t)))
-  | beta_pr {Γ: Context} {φ A s t: Term}:
+  | beta_pr {Γ: Context} {φ A s p: Term}:
     HasType ((Hyp.mk φ (HypKind.val prop))::Γ) s (term A) ->
     HasType Γ φ prop ->
     HasType Γ.upgrade p (proof φ) ->
     HasType Γ (beta_pr p s) 
-    (proof (eq (A.subst0 t) 
+    (proof (eq (A.subst0 p) 
     (app_pr (assume φ A) (lam_pr φ s) p) (s.subst0 p)))
   | beta_ir {Γ: Context} {A B s t: Term}:
     HasType ((Hyp.mk A HypKind.gst)::Γ) s (term B) ->
