LogicalRefinement/Typed/Regular.lean
@@ -165,7 +165,22 @@ theorem HasType.regular (p: Γ ⊢ a: A): A.regular Γ := by {
       exact Ht.upgrade.upgrade
       exact Hs.upgrade.upgrade.subst0 Ht.upgrade
 
-  case beta_pr => sorry
+  case beta_pr Hs Hφ Hp Is _ _  => 
+    cases Is with
+    | expr HA =>
+      constructor
+      apply HasType.downgrade
+      constructor
+      exact HA.upgrade.subst0_sort Hp
+      constructor
+      constructor
+      exact Hφ.upgrade.upgrade
+      exact HA.upgrade.upgrade
+      constructor
+      exact Hφ.upgrade.upgrade
+      exact Hs.upgrade.upgrade
+      exact Hp.upgrade
+      exact Hs.upgrade.upgrade.subst0 Hp.upgrade
 
   case eta Γ A B f Hf _ If _ => 
     cases If with
